Enable canonical `fun _ => _` projections.

pretyping/evarconv.ml
@@ -244,7 +244,10 @@ let check_conv_record env sigma (t1,sk1) (t2,sk2) =
   let canon_s,sk2_effective =
     try
       match EConstr.kind sigma t2 with
-        Prod (_,a,b) -> (* assert (l2=[]); *)
+      | Lambda (_,_,_) -> (* assert (l2=[]); *)
+        lookup_canonical_conversion (proji, Lambda_cs),
+        (Stack.append_app [|t2|] Stack.empty)
+      | Prod (_,a,b) -> (* assert (l2=[]); *)
           let _, a, b = destProd sigma t2 in
           if noccurn sigma 1 b then
             lookup_canonical_conversion (proji, Prod_cs),
