pretyping/recordops.ml
@@ -149,6 +149,7 @@ type obj_typ = {
 
 type cs_pattern =
     Const_cs of GlobRef.t
+  | Lambda_cs
   | Prod_cs
   | Sort_cs of Sorts.family
   | Default_cs
@@ -156,6 +157,7 @@ type cs_pattern =
 let eq_cs_pattern p1 p2 = match p1, p2 with
 | Const_cs gr1, Const_cs gr2 -> GlobRef.equal gr1 gr2
 | Prod_cs, Prod_cs -> true
+| Lambda_cs, Lambda_cs -> true
 | Sort_cs s1, Sort_cs s2 -> Sorts.family_equal s1 s2
 | Default_cs, Default_cs -> true
 | _ -> false
@@ -183,6 +185,7 @@ let rec cs_pattern_of_constr env t =
     let patt, n, args = cs_pattern_of_constr env f in
     patt, n, args @ Array.to_list vargs
   | Rel n -> Default_cs, Some n, []
+  | Lambda (_, _, _) -> Lambda_cs, None, [t]
   | Prod (_,a,b) when Vars.noccurn 1 b -> Prod_cs, None, [a; Vars.lift (-1) b]
   | Proj (p, c) ->
     let { Environ.uj_type = ty } = Typeops.infer env c in
@@ -243,6 +246,7 @@ let compute_canonical_projections env ~warn (gref,ind) =
 
 let pr_cs_pattern = function
     Const_cs c -> Nametab.pr_global_env Id.Set.empty c
+  | Lambda_cs -> str "fun _ => _"
   | Prod_cs -> str "_ -> _"
   | Default_cs -> str "_"
   | Sort_cs s -> Sorts.pr_sort_family s
