pretyping/recordops.mli
@@ -68,6 +68,7 @@ val find_primitive_projection : Constant.t -> Projection.Repr.t option
 (** A cs_pattern characterizes the form of a component of canonical structure *)
 type cs_pattern =
     Const_cs of GlobRef.t
+  | Lambda_cs
   | Prod_cs
   | Sort_cs of Sorts.family
   | Default_cs
